introduced core trans specs, revised interface

coreIfScript.sml
@@ -23,12 +23,36 @@ val _ = Datatype `core_state =
 
 val _ = Datatype `resource = REG reg_name | COREG coreg_name | 
 		             PSRS psrs_name | MEM padr`;
+val reg_res_def = Define `
+   (reg_res (MEM pa) = F)
+/\ (reg_res _ = T)
+`;
+
+val res_cases = store_thm("res_cases", ``
+!r. (?pa. r = MEM pa) /\ ~reg_res r
+ \/ (!pa. r <> MEM pa) /\ reg_res r
+``,
+  Cases >> (
+      RW_TAC std_ss [reg_res_def]
+  )
+);
+
 val CV_def = Define `
    (CV c (mv:mem_view) (REG r) = c.reg r)
 /\ (CV c mv (COREG r) = c.coreg r)
 /\ (CV c mv (PSRS r) = c.psrs r)
 /\ (CV c mv (MEM pa) = mv T pa)
 `;
+
+val CV_reg_lem = store_thm("CV_reg_lem", ``
+!c mv mv' r. reg_res r ==> (CV c mv r = CV c mv' r)
+``,
+  REPEAT STRIP_TAC >>
+  Cases_on `r` >> (
+      FULL_SIMP_TAC std_ss [reg_res_def, CV_def]
+  )   
+);
+
 
 val CR_exists = prove (``
 ?CR:core_state # mem_view -> resource set.
@@ -49,8 +73,6 @@ new_constant("MODE", ``:(psrs_name -> word) -> mode``);
 
 val Mode_def = Define `Mode c = MODE c.psrs`; 
 val Pc_def = Define `Pc c = c.reg PC`; 
-
-new_constant("CR", ``:core_state -> mem_view -> resource set``);
 
 (* Monitor spec *)
 
@@ -77,25 +99,138 @@ val dummyMon_def = Define `
 
 val Mon_exists = prove (``
 ?(Mon:core_state # mem_view # resource # mode # acc -> bool).
-!c mv pa m ac. (?va ca. Mmu_(c,mv,va,m,ac) = SOME(pa,ca)) <=>
-               Mon(c,mv,MEM pa,m,ac)
+!c mv ac. 
+   (!pa m. (?va ca. Mmu_(c,mv,va,m,ac) = SOME(pa,ca)) <=> Mon(c,mv,MEM pa,m,ac))
+/\ (!r. reg_res r /\ r IN MD_ (c,mv) ==> ~Mon(c,mv,r,USER,ac))
+/\ (!r mv' m. reg_res r ==> (Mon(c,mv,r,m,ac) = Mon(c,mv',r,m,ac)))
 ``,
   EXISTS_TAC ``dummyMon`` >>
-  RW_TAC std_ss [dummyMon_def]
+  RW_TAC std_ss [dummyMon_def] >>
+  Cases_on `r` >> (
+      FULL_SIMP_TAC std_ss [reg_res_def] >>
+      RW_TAC std_ss [dummyMon_def]
+  )  
 );  
 
 val Mon_spec = new_specification ("Mon_spec",
   ["Mon_"], Mon_exists);
 
-(* transition relations, TODO: replace with specs, when requirements known *)
+(* exception entry point *)
 
-val _ = new_constant("core_req", 
-		     ``:core_state # mode # corereq # core_state -> bool``
-);
+val dummyexentry_def = Define `dummyexentry c = (Mode c = PRIV)`;
 
-val _ = new_constant("core_rcv", 
-		     ``:core_state # mode # word # core_state -> bool``
-);
+val exentry_exists = prove (``
+?exentry:core_state -> bool. !c. exentry c ==> (Mode c = PRIV)
+``,
+  EXISTS_TAC ``dummyexentry`` >>
+  RW_TAC std_ss [dummyexentry_def]
+);  
+
+val exentry_spec = new_specification ("exentry_spec",
+  ["exentry_"], exentry_exists);
+
+(***** transition relations *****)
+
+(* requesting transition *)
+
+val core_mode_po = Define `core_mode_po trans = 
+!c M mv req c'. trans (c,M,mv,req,c') ==> (Mode c = M)
+`;
+
+(* change to PRIV -> exentry *)
+val core_exentry_po = Define `core_exentry_po trans = 
+!c mv req c'. trans (c,USER,mv,req,c') /\ (Mode c' = PRIV) ==> 
+    exentry_ c' /\ (req = NOREQ)
+`;
+
+(* mem request -> Mon obeyed *)
+val core_Mon_mem_po = Define `core_Mon_mem_po trans = 
+!c M mv req c'. trans (c,M,mv,req,c') /\ (req <> NOREQ) ==> 
+    Mon_(c,mv,MEM (Adr req),M,Acc req)
+`;
+
+(* reg unchanged if no Mon permission *)
+val core_Mon_reg_po = Define `core_Mon_reg_po trans = 
+!c M mv req r c'. reg_res r /\ trans (c,M,mv,req,c') /\ ~Mon_(c,mv,r,M,W) ==>
+    (CV c mv r = CV c' mv r)
+`;
+
+(* corereq only depending on MD in memview *)
+val core_MD_mv_po = Define `core_MD_mv_po trans = 
+!c M mv mv' req c'. (!r. r IN MD_ (c,mv) ==> (CV c mv r = CV c mv' r)) ==>
+    (trans (c,M,mv,req,c') <=> trans (c,M,mv',req,c'))
+`;
+
+val dummy_cr_def = Define `
+dummy_cr (c:core_state,M:mode,mv:mem_view,req:corereq,c':core_state) = 
+(c = c') /\ (req = NOREQ) /\ (Mode c = M)
+`;
+
+val core_req_exists = prove (``
+?(trans:core_state # mode # mem_view # corereq # core_state -> bool).
+    core_mode_po trans
+ /\ core_exentry_po trans
+ /\ core_Mon_mem_po trans
+ /\ core_Mon_reg_po trans
+ /\ core_MD_mv_po trans
+``,
+  EXISTS_TAC ``dummy_cr`` >>
+  REPEAT STRIP_TAC 
+  >| [(* mode *)
+      RW_TAC std_ss [core_mode_po, dummy_cr_def]
+      ,
+      (* exentry *)
+      RW_TAC std_ss [core_exentry_po, dummy_cr_def] >>
+      FULL_SIMP_TAC std_ss [mode_distinct]
+      ,
+      (* memory monitor *)
+      RW_TAC std_ss [core_Mon_mem_po, dummy_cr_def]
+      ,
+      (* reg monitor *)
+      RW_TAC std_ss [core_Mon_reg_po, dummy_cr_def]
+      ,
+      (* MD dependency *)
+      RW_TAC std_ss [core_MD_mv_po, dummy_cr_def]
+     ]
+);  
+
+val core_req_spec = new_specification ("core_req_spec",
+  ["core_req"], core_req_exists);
+
+(* receiving transition, for receiving read results *)
+
+(* does not change mode *)
+val rcv_mode_po = Define `rcv_mode_po trans = 
+!c M w c'. trans (c,M,w,c') ==> (Mode c = M) /\ (Mode c = Mode c')
+`;
+
+val rcv_Mon_reg_po = Define `rcv_Mon_reg_po trans = 
+!c M w mv r c'. reg_res r /\ trans (c,M,w,c') /\ ~Mon_(c,mv,r,M,W) ==>
+    (CV c mv r = CV c' mv r)
+`;
+
+val dummy_rcv_def = Define `
+dummy_rcv (c:core_state,M:mode,w:word,c':core_state) = 
+(c = c') /\ (Mode c = M)
+`;
+
+val core_rcv_exists = prove (``
+?(trans:core_state # mode # word # core_state -> bool).
+    rcv_mode_po trans
+ /\ rcv_Mon_reg_po trans
+``,
+  EXISTS_TAC ``dummy_rcv`` >>
+  REPEAT STRIP_TAC 
+  >| [(* mode *)
+      RW_TAC std_ss [rcv_mode_po, dummy_rcv_def]
+      ,
+      (* reg monitor *)
+      RW_TAC std_ss [rcv_Mon_reg_po, dummy_rcv_def]
+     ]
+);  
+
+val core_rcv_spec = new_specification ("core_rcv_spec",
+  ["core_rcv"], core_rcv_exists);
 
 (* Proof obligations on components, exported to main theory *)
 
